examples/bloomfilter/verif.v
@@ -5,7 +5,8 @@ Open Scope string_scope.
 
 Import ListNotations.
 Require Import ProD3.examples.bloomfilter.p4ast.
-Require Import ProD3.examples.bloomfilter.bloomfilter.
+Require Import ProD3.examples.sbf.ConFilter.
+Require Import ProD3.examples.sbf.general_bf.
 
 Require Import Poulet4.Utils.Maps.
 Require Import Poulet4.P4light.Semantics.Semantics.
@@ -58,26 +59,18 @@ Open Scope func_spec.
 
 (* Bloom filter encoding *)
 
-Notation Filter := (Filter Z).
+Notation Filter := row.
 
-Definition bloomfilter_state : Type := Filter * Filter * Filter.
+Definition bloomfilter_state : Type := frame.
 
 Definition bool_to_Z (b : bool) :=
   if b then 1 else 0.
 
-Definition list_of_filter (size : Z) (f : Filter) : list Z :=
-  map (compose bool_to_Z (compose f Z.of_nat)) (seq O (Z.to_nat size)).
+Definition list_of_filter (f : Filter) : list Z := map bool_to_Z f.
 
 Definition NUM_ENTRY : Z := 1024.
 
-Definition bloom0 (bst : bloomfilter_state) : list Z :=
-  list_of_filter NUM_ENTRY (fst (fst bst)).
-
-Definition bloom1 (bst : bloomfilter_state) : list Z :=
-  list_of_filter NUM_ENTRY (snd (fst bst)).
-
-Definition bloom2 (bst : bloomfilter_state) : list Z :=
-  list_of_filter NUM_ENTRY (snd bst).
+Definition blooms (bst: bloomfilter_state) : list (list Z) := map list_of_filter bst.
 
 Definition reg_encode (l : list Z) : extern_object :=
   ObjRegister (map ValBaseBit (map (P4Arith.to_lbool 1) l)).
@@ -106,9 +99,11 @@ Qed.
 
 Hint Rewrite Znth_seq using lia : Znth.
 
-Lemma Zlength_list_of_filter : forall n filter,
-  0 <= n ->
-  Zlength (list_of_filter n filter) = n.
+Definition bf_wellformed (bst: bloomfilter_state) :=
+  Zlength bst = 3 /\ Forall (fun r => Zlength r = NUM_ENTRY) bst.
+
+Lemma Zlength_list_of_filter : forall filter,
+  Zlength (list_of_filter filter) = Zlength filter.
 Proof.
   intros.
   unfold list_of_filter.
@@ -117,45 +112,41 @@ Qed.
 
 Hint Rewrite Zlength_list_of_filter using lia : Zlength.
 
-Lemma Znth_list_of_filter : forall n filter i,
-  0 <= i < n ->
-  Znth i (list_of_filter n filter) = bool_to_Z (filter i).
+Lemma Znth_list_of_filter : forall filter i,
+  0 <= i < Zlength filter ->
+  Znth i (list_of_filter filter) = bool_to_Z (Znth i filter).
 Proof.
   intros.
   unfold list_of_filter.
   list_simplify.
-  unfold compose.
-  do 2 f_equal. lia.
 Qed.
 
 Hint Rewrite Znth_list_of_filter using lia : Znth.
 
 Lemma update_bit : forall filter hash,
-  reg_encode (list_of_filter NUM_ENTRY (upd Z Z.eqb filter hash true)) =
+  reg_encode (list_of_filter (row_insert filter hash)) =
   ObjRegister
-    (upd_Znth hash (map ValBaseBit (map (to_lbool 1) (list_of_filter NUM_ENTRY filter)))
+    (upd_Znth hash (map ValBaseBit (map (to_lbool 1) (list_of_filter filter)))
        (ValBaseBit (to_lbool 1 (BitArith.mod_bound 1 1)))).
 Proof.
   intros.
   unfold reg_encode.
   f_equal.
-  unfold upd.
-  unfold NUM_ENTRY.
+  unfold row_insert.
   list_simplify.
-  - replace (hash =? i) with true by lia.
-    reflexivity.
-  - replace (hash =? i) with false by lia.
-    reflexivity.
+  - subst.
+    rewrite Znth_list_of_filter; list_solve.
+  - rewrite Znth_list_of_filter; list_solve.
 Qed.
 
 Lemma get_bit : forall (filter : Filter) hash,
-  0 <= hash < NUM_ENTRY ->
-  Znth hash (map ValBaseBit (map (to_lbool 1) (list_of_filter NUM_ENTRY filter)))
-    = ValBaseBit [filter hash].
+  0 <= hash < Zlength filter ->
+  Znth hash (map ValBaseBit (map (to_lbool 1) (list_of_filter filter)))
+    = ValBaseBit [Znth hash filter].
 Proof.
   intros.
   list_simplify.
-  destruct (filter hash); reflexivity.
+  destruct (Znth hash filter); reflexivity.
 Qed.
 
 Definition Add_fundef := Eval compute in
@@ -167,12 +158,6 @@ Section CRC.
 Import Hexadecimal.
 
 Definition CRC : list bool -> list bool := Hash.compute_crc 16%nat (D8 (D0 (D0 (D5 Nil)))) zero zero true true.
-
-(* This may be unnecessary. *)
-Lemma CRC_length : forall data,
-  List.length (CRC data) = 16%nat.
-Proof.
-Admitted.
 
 End CRC.
 
@@ -199,16 +184,16 @@ Definition bloomfilter_exts := [["bloom0"]; ["bloom1"]; ["bloom2"]].
 
 Definition encode_bloomfilter_state bf : ext_pred :=
   ExtPred.and
-    (ExtPred.singleton ["bloom0"] (reg_encode (bloom0 bf)))
+    (ExtPred.singleton ["bloom0"] (reg_encode (Znth 0 (blooms bf))))
     (ExtPred.and
-      (ExtPred.singleton ["bloom1"] (reg_encode (bloom1 bf)))
-      (ExtPred.singleton ["bloom2"] (reg_encode (bloom2 bf)))).
+      (ExtPred.singleton ["bloom1"] (reg_encode (Znth 1 (blooms bf))))
+      (ExtPred.singleton ["bloom2"] (reg_encode (Znth 2 (blooms bf))))).
 
 Definition bloomfilter_add bf data :=
-  bloomfilter.add Z Z.eqb CRC_pad0 CRC_pad1 CRC_pad2 bf data.
+  general_bf.add [CRC_pad0; CRC_pad1; CRC_pad2] bf data.
 
 Definition bloomfilter_query bf data :=
-  bloomfilter.query Z CRC_pad0 CRC_pad1 CRC_pad2 bf data.
+  general_bf.query [CRC_pad0; CRC_pad1; CRC_pad2] bf data.
 
 Definition havoc_typ (typ : @P4Type Info) : Sval :=
   force ValBaseNull (uninit_sval_of_typ None typ).
@@ -321,7 +306,7 @@ Definition Add_spec : func_spec :=
   WITH p,
     PATH p
     MOD None bloomfilter_exts
-    WITH (data : Z) (bf : bloomfilter_state),
+    WITH (data : Z) (bf : bloomfilter_state) (H_bf: bf_wellformed bf),
       PRE
         (ARG [myHeader_encode data; havoc_typ custom_metadata_t]
         (MEM []
@@ -335,6 +320,8 @@ Lemma Add_body : fundef_satisfies_spec ge Add_fundef nil Add_spec.
 Proof.
   unfold Add_spec, bloomfilter_exts.
   start_function.
+  destruct H_bf. do 3 (destruct bf; [exfalso; list_solve |]).
+  destruct bf; [|exfalso; list_solve].
   step_call hash_body [ValBaseBit (to_lbool 16 data); ValBaseBit (to_lbool 3 3)].
   2 : entailer.
   reflexivity.
@@ -365,7 +352,8 @@ Proof.
   step.
   entailer.
   { repeat constructor. }
-  all : destruct bf as [[] ?]; symmetry; apply update_bit.
+  all: unfold blooms, bloomfilter_add, add, frame_insert, Utils.map2;
+    cbn [map combine uncurry]; symmetry; apply update_bit.
 Qed.
 
 #[local] Hint Extern 5 (func_modifies _ _ _ _ _) => (apply Add_body) : func_specs.
@@ -377,7 +365,7 @@ Definition Query_spec : func_spec :=
   WITH p,
     PATH p
     MOD None []
-    WITH (data : Z) (bf : bloomfilter_state),
+    WITH (data : Z) (bf : bloomfilter_state) (H_bf: bf_wellformed bf),
       PRE
         let hdr := ValBaseStruct
         [("myHeader",
@@ -394,11 +382,20 @@ Definition Query_spec : func_spec :=
             [("data", ValBaseBit (to_loptbool 16 data))]
              (Some true))] in
         let meta := update "member0"
-          (ValBaseBit [Some (bloomfilter.query Z CRC_pad0 CRC_pad1 CRC_pad2 bf data)])
+          (ValBaseBit [Some (general_bf.query [CRC_pad0; CRC_pad1; CRC_pad2] bf data)])
           (force ValBaseNull (uninit_sval_of_typ None custom_metadata_t)) in
         (ARG_RET [hdr; meta] ValBaseNull
         (MEM []
-        (EXT []))).
+           (EXT []))).
+
+Lemma Znth_0_3 {X: Type} {HX: Inhabitant X}: forall (r0 r1 r2: X), Znth 0 [r0; r1; r2] = r0.
+Proof. intros. now vm_compute. Qed.
+
+Lemma Znth_1_3 {X: Type} {HX: Inhabitant X}: forall (r0 r1 r2: X), Znth 1 [r0; r1; r2] = r1.
+Proof. intros. now vm_compute. Qed.
+
+Lemma Znth_2_3 {X: Type} {HX: Inhabitant X}: forall (r0 r1 r2: X), Znth 2 [r0; r1; r2] = r2.
+Proof. intros. now vm_compute. Qed.
 
 Lemma Query_body : fundef_satisfies_spec ge Query_fundef nil Query_spec.
 Proof.
@@ -432,20 +429,23 @@ Proof.
   { apply CRC_range. }
   step.
   step.
-  destruct bf as [[f0 f1] f2].
-  unfold bloom0.
-  unfold bloom1.
-  unfold bloom2.
-  rewrite !get_bit by (apply CRC_range).
+  destruct H_bf. do 3 (destruct bf; [exfalso; list_solve |]).
+  destruct bf; [|exfalso; list_solve]. rewrite Forall_forall in H0.
+  assert (Zlength r = NUM_ENTRY) by (apply H0; now left).
+  assert (Zlength r0 = NUM_ENTRY) by (apply H0; right; now left).
+  assert (Zlength r1 = NUM_ENTRY) by (apply H0; right; right; now left).
+  unfold blooms. cbn [map]. rewrite Znth_0_3, Znth_1_3, Znth_2_3.
+  rewrite !get_bit by (first [rewrite H1 | rewrite H2 | rewrite H3]; apply CRC_range).
   entailer.
   { simpl build_abs_unary_op.
-    unfold query, bloomfilter.get.
-    simpl.
-    destruct (f0 (CRC_pad0 data));
-      destruct (f1 (CRC_pad1 data));
-      destruct (f2 (CRC_pad2 data));
-      repeat constructor.
-  }
+    replace (query [CRC_pad0; CRC_pad1; CRC_pad2] [r; r0; r1] data) with
+      (Znth (CRC_pad0 data) r && Znth (CRC_pad1 data) r0 && Znth (CRC_pad2 data) r1).
+    2: { unfold query, frame_query, Utils.fold_andb, Utils.map2, row_query.
+         cbn [map combine uncurry fold_left]. auto. }
+    destruct (Znth (CRC_pad0 data) r);
+      destruct (Znth (CRC_pad1 data) r0);
+      destruct (Znth (CRC_pad2 data) r1);
+      simpl; repeat constructor. }
 Qed.
 
 #[local] Hint Extern 5 (func_modifies _ _ _ _ _) => (apply Query_body) : func_specs.
@@ -455,15 +455,15 @@ Definition MyIngress_fundef := Eval compute in
 
 Definition process (in_port data : Z) (bf : bloomfilter_state) : (bloomfilter_state * Z) :=
   if in_port =? 0 then
-    (bloomfilter.add Z Z.eqb CRC_pad0 CRC_pad1 CRC_pad2 bf data, 1)
+    (general_bf.add [CRC_pad0; CRC_pad1; CRC_pad2] bf data, 1)
   else
-    (bf, if bloomfilter.query Z CRC_pad0 CRC_pad1 CRC_pad2 bf data then 0 else 511).
+    (bf, if general_bf.query [CRC_pad0; CRC_pad1; CRC_pad2] bf data then 0 else 511).
 
 Definition bloomfilter_spec : func_spec :=
   WITH ,
     PATH ["main"; "ig"]
     MOD None bloomfilter_exts
-    WITH in_port data bf (H : 0 <= in_port < 2),
+    WITH in_port data bf (H : 0 <= in_port < 2) (H_bf: bf_wellformed bf),
       PRE
         (ARG [
           ValBaseStruct [("myHeader",
@@ -513,7 +513,7 @@ Proof.
     assert (in_port = 0) by lia; subst. clear H_in_port.
     step.
     step.
-    step_call Add_body.
+    step_call Add_body. eauto.
     entailer.
     step.
     entailer.
@@ -533,12 +533,12 @@ Proof.
     simpl (force empty_statement _).
     step.
     step.
-    step_call Query_body.
+    step_call Query_body. eauto.
     entailer.
     step_if.
     {
       rewrite get_update_same in H0 by auto.
-      destruct (query Z CRC_pad0 CRC_pad1 CRC_pad2 bf data) eqn:H_query; inv H0.
+      destruct (query [CRC_pad0; CRC_pad1; CRC_pad2] bf data) eqn:H_query; inv H0.
       step.
       step.
       step.
@@ -550,7 +550,7 @@ Proof.
     }
     {
       rewrite get_update_same in H0 by auto.
-      destruct (query Z CRC_pad0 CRC_pad1 CRC_pad2 bf data) eqn:H_query; inv H0.
+      destruct (query [CRC_pad0; CRC_pad1; CRC_pad2] bf data) eqn:H_query; inv H0.
       simpl (force empty_statement _).
       step.
       step.
